IT WORKS

examples/Fuzz.v
@@ -2,6 +2,77 @@ From QuickChick Require Import QuickChick.
 Import MonadNotation.
 Require Import Arith.
 
+Inductive Tree :=
+| Leaf : Tree
+| Node : nat -> Tree -> Tree -> Tree.
+
+#[local] Instance MutateNat : Mutate nat :=
+  {| mutate n := choose (n - 5, n + 5) |}.
+
+#[local] Instance FuzzyNat : Fuzzy nat :=
+  {| fuzz n := choose (n - 5, n + 5) |}.
+
+Derive (Arbitrary, Show, Sized, Mutate) for Tree.
+
+QuickChickDebug Debug On.
+Derive Fuzzy for Tree.
+
+Inductive bst : nat -> nat -> Tree -> Prop :=
+| bst_leaf : forall lo hi, bst lo hi Leaf
+| bst_node : forall lo hi x l r,
+    le (S lo) x ->  le (S x) hi ->
+    bst lo x l -> bst x hi r ->
+    bst lo hi (Node x l r).
+
+Derive DecOpt for (le x y).
+
+Derive ArbitrarySizedSuchThat for (fun x => le y x).
+Derive ArbitrarySizedSuchThat for (fun t => bst lo hi t).
+
+Derive DecOpt for (bst lo hi t).
+
+Fixpoint is_bst (lo hi : nat) (t : Tree) :=
+  match t with
+  | Leaf => true
+  | Node x l r =>
+    andb ((lo < x /\ x < hi) ?)
+         (andb (is_bst lo x l)
+               (is_bst x hi r))
+  end.
+
+Fixpoint insert (x : nat) (t : Tree) :=
+  match t with
+  | Leaf => Node x Leaf Leaf
+  | Node y l r =>
+    if x < y ? then
+      Node y (insert x l) r
+    else if x > y ? then
+      Node y l (insert x r)
+    else t
+  end.
+
+Fixpoint mem (x : nat) (t : Tree) :=
+  match t with
+  | Leaf => false
+  | Node y l r =>
+      orb (x =? y) (mem x l)
+  end.
+
+(*
+Definition bst_checker_prop :=
+  forAllMaybe (genST (fun t => bst 0 17 t)) (fun t => 
+  forAll (choose (1, 16)) (fun x => 
+  bst 0 17 (insert x t) ?? 10)). (* *)
+(*  is_bst 0 17 (insert x t))). *)
+
+Extract Constant defNumTests => "20000".
+QuickChick bst_checker_prop. 
+*)
+
+Definition prop (t : Tree) :=
+  Some (mem 4 (insert 4 t)).
+
+(*
 Definition test_prop (n : nat) := Some (n <=? 10).
 
 Definition gen : G nat := choose (0,5).
@@ -9,9 +80,18 @@ Definition gen : G nat := choose (0,5).
 Definition fuzz (n : nat) : G nat :=
   x <- choose (1,3);;
   ret (n + x).
+ *)
 
+QuickChick prop.
+
+ManualExtract Tree.
 Definition fuzzer :=
-  fun (u : unit) => fuzzLoop gen fuzz show test_prop.
+  fun (u : unit) => fuzzLoop arbitrary mutate show prop.
 
+FuzzChick prop (fuzzer tt).
 QuickChickDebug Debug On.
-FuzzChick test_prop (fuzzer tt).
+
+Definition fuzz_fuzzer :=
+  fun (u : unit) => fuzzLoop arbitrary fuzz show prop.
+
+(* FuzzChick prop (fuzz_fuzzer tt). *)
